Prove almost sure termination of BernoulliExpNeg
Currently, this assumes measurability and independence.

src/Distributions/BernoulliExpNeg/Model.dfy
@@ -5,10 +5,15 @@
 
 module BernoulliExpNeg.Model {
   import Rationals
+  import RealArith
+  import Sequences
+  import Limits
+  import Measures
   import Rand
   import Uniform
   import Bernoulli
   import Monad
+  import Independence
   import Loops
   import BernoulliModel = Bernoulli.Model
 
@@ -33,6 +38,7 @@ module BernoulliExpNeg.Model {
   ghost function SampleLe1(gamma: Rationals.Rational): Monad.Hurd<bool>
     requires 0 <= gamma.numer <= gamma.denom
   {
+    // TODO: replace with Map
     Monad.Bind(
       Le1Loop(gamma)((true, 0)),
       (ak: (bool, nat)) => Monad.Return(ak.1 % 2 == 1)
@@ -58,6 +64,7 @@ module BernoulliExpNeg.Model {
   {
     (ak: (bool, nat)) =>
       var k' := ak.1 + 1;
+      // TODO: should be Map
       Monad.Bind(
         BernoulliModel.Sample(gamma.numer, k' * gamma.denom),
         SetK(k'))
@@ -67,9 +74,185 @@ module BernoulliExpNeg.Model {
     a => Monad.Return((a, k))
   }
 
-  lemma {:axiom} Le1LoopTerminatesAlmostSurely(gamma: Rationals.Rational)
+  lemma {:axiom} Le1LoopIterCorrectness(gamma: Rationals.Rational, ak: (bool, nat), k': nat) // TODO
+    requires k' == ak.1 + 1
+    requires 0 <= gamma.numer <= gamma.denom
+    ensures Rand.prob(Monad.BitstreamsWithValueIn(Le1LoopIter(gamma)(ak), iset{(true, k')})) == gamma.numer as real / (k' * gamma.denom) as real
+    ensures Rand.prob(Monad.BitstreamsWithValueIn(Le1LoopIter(gamma)(ak), iset{(false, k')})) == 1.0 - gamma.numer as real / (k' * gamma.denom) as real
+
+  ghost function Le1LoopDivergenceProbBound(k: nat): nat -> real {
+    (fuel: nat) => if fuel == 0 then 1.0 else 1.0 / (k + fuel) as real
+  }
+
+  /* Proves that Le1Loop terminates almost surely.
+   *
+   * It does so by bounding the probability of nontermination (divergence) after `fuel` iterations between 0.0 and `Le1LoopDivergenceProbBound(k)(fuel)`.
+   * Since both lower and upper bounds converge to zero as `fuel` tends to infinity, the divergence probability is zero.
+  */
+  lemma Le1LoopTerminatesAlmostSurely(gamma: Rationals.Rational)
     requires 0 <= gamma.numer <= gamma.denom
     ensures Loops.WhileTerminatesAlmostSurely(Le1LoopCondition, Le1LoopIter(gamma))
+  {
+    var divergenceLower := Sequences.Constant(0.0);
+    forall init: (bool, nat) ensures Loops.WhileTerminatesAlmostSurelyInit(Le1LoopCondition, Le1LoopIter(gamma), init) {
+      var divergenceProb := Loops.WhileCutDivergenceProbability(Le1LoopCondition, Le1LoopIter(gamma), init);
+      assert Sequences.IsLeq(divergenceProb, Le1LoopDivergenceProbBound(0)) by {
+        forall fuel: nat ensures divergenceProb(fuel) <= Le1LoopDivergenceProbBound(0)(fuel) {
+          Le1LoopDivergenceProbabilityBound(gamma, init, fuel);
+          assert divergenceProb(fuel) <= Le1LoopDivergenceProbBound(init.1)(fuel) <= Le1LoopDivergenceProbBound(0)(fuel) by {
+            if fuel > 0 {
+              RealArith.DivisionIsAntiMonotonic(1.0, (fuel + init.1) as real, fuel as real);
+            }
+          }
+        }
+      }
+      assert Limits.ConvergesTo(Le1LoopDivergenceProbBound(0), 0.0) by {
+        assert Sequences.IsSuffixOf(Sequences.OneOverNPlus1, Le1LoopDivergenceProbBound(0), 1);
+        Limits.OneOverNPlus1ConvergesToZero();
+        Limits.SuffixConvergesToSame(Le1LoopDivergenceProbBound(0), Sequences.OneOverNPlus1, 1, 0.0);
+      }
+      assert Sequences.IsLeq(divergenceLower, divergenceProb) by {
+        forall n: nat ensures divergenceProb(n) >= 0.0 {
+          Rand.ProbIsProbabilityMeasure();
+          var event := iset s | !Loops.WhileCutTerminatesWithFuel(Le1LoopCondition, Le1LoopIter(gamma), init, s)(n);
+          assume {:axiom} event in Rand.eventSpace; // TODO
+          assert Rand.prob(event) >= 0.0;
+        }
+      }
+      assert Limits.ConvergesTo(divergenceLower, 0.0) by {
+        Limits.ConstantSequenceConverges(divergenceLower, 0.0);
+      }
+      assert Limits.ConvergesTo(divergenceProb, 0.0) by {
+        Limits.Sandwich(divergenceLower, divergenceProb, Le1LoopDivergenceProbBound(0), 0.0);
+      }
+      Loops.EnsureWhileTerminatesAlmostSurelyViaLimit(Le1LoopCondition, Le1LoopIter(gamma), init);
+    }
+  }
 
+  /* Proves a bound on the nontermination (divergence) probability of Le1Loop(gamma)(ak) after `n` iterations.
+   *
+   * We could prove an even stronger bound of (gamma / (k + 1)) * (gamma / (k + 2)) * ... * (gamma / (k + n)),
+   * where k = ak.1.
+   * But such a bound is more complicated to express, so we instead prove the upper bound 1 if n = 0 and 1 / (k + n) else.
+   *
+   * We do this inductively.
+   * For n = 0 the bound of 1 is clear.
+   * For n >= 1, we reason as follows:
+   * If ak.0 is false, the loop stops and the divergence probability is zero.
+   * So the interesting case is ak.0 == true.
+   * If n == 1, the probability of sampling true from the Bernoulli(gamma / (k + 1)) distribution is <= 1 / (k + 1) == 1 / (k + n).
+   * Since the loop exits if we sample false, this is an upper bound on the divergence probability.
+   * If n > 1, the probability of divergence is at most that of the remaining n - 1 loop iterations diverging.
+   * By induction hypothesis, this is <= 1 / (k' + n - 1) == 1 / (k + n) as desired.
+  */
+  lemma Le1LoopDivergenceProbabilityBound(gamma: Rationals.Rational, ak: (bool, nat), n: nat)
+    requires 0 <= gamma.numer <= gamma.denom
+    decreases n
+    ensures Loops.WhileCutDivergenceProbability(Le1LoopCondition, Le1LoopIter(gamma), ak)(n) <= Le1LoopDivergenceProbBound(ak.1)(n)
+  {
+    var divergenceEvent := iset s | !Loops.WhileCutTerminatesWithFuel(Le1LoopCondition, Le1LoopIter(gamma), ak, s)(n);
+    assume {:axiom} divergenceEvent in Rand.eventSpace;
+    if n == 0 {
+      assert Loops.WhileCutDivergenceProbability(Le1LoopCondition, Le1LoopIter(gamma), ak)(n) == Rand.prob(divergenceEvent);
+      Rand.ProbIsProbabilityMeasure();
+      Measures.ProbabilityLe1(divergenceEvent, Rand.eventSpace, Rand.prob);
+      assert Loops.WhileCutDivergenceProbability(Le1LoopCondition, Le1LoopIter(gamma), ak)(n) <= Le1LoopDivergenceProbBound(ak.1)(n);
+    } else {
+      if !Le1LoopCondition(ak) {
+        forall s ensures Loops.WhileCutTerminatesWithFuel(Le1LoopCondition, Le1LoopIter(gamma), ak, s)(n) {}
+        assert Loops.WhileCutDivergenceProbability(Le1LoopCondition, Le1LoopIter(gamma), ak)(n) == 0.0 by {
+          assert iset{} == iset s | !Loops.WhileCutTerminatesWithFuel(Le1LoopCondition, Le1LoopIter(gamma), ak, s)(n);
+          Rand.ProbIsProbabilityMeasure();
+        }
+      } else {
+      var (a, k) := ak;
+      var k': nat := k + 1;
+      var continueValues := iset ak': (bool, nat) | Le1LoopCondition(ak');
+      var firstIterationContinuesEvent := Monad.BitstreamsWithValueIn(Le1LoopIter(gamma)(ak), continueValues);
+      var restOfLoopDiverges := iset s | !Loops.WhileCutTerminatesWithFuel(Le1LoopCondition, Le1LoopIter(gamma), (true, k'), s)(n - 1);
+      assume {:axiom} firstIterationContinuesEvent in Rand.eventSpace; // TODO
+      assume {:axiom} restOfLoopDiverges in Rand.eventSpace; // TODO
+      assert divergenceEvent == firstIterationContinuesEvent * Monad.BitstreamsWithRestIn(Le1LoopIter(gamma)(ak), restOfLoopDiverges) by {
+        forall s ensures s in divergenceEvent <==> s in firstIterationContinuesEvent && s in Monad.BitstreamsWithRestIn(Le1LoopIter(gamma)(ak), restOfLoopDiverges) {
+          match Le1LoopIter(gamma)(ak)(s)
+          case Diverging => {}
+          case Result(ak', s') =>
+            assert s in firstIterationContinuesEvent <==> ak'.0;
+            if ak'.0 {
+              assert ak' == (true, k');
+              calc {
+                s in divergenceEvent;
+                !Loops.WhileCutTerminatesWithFuel(Le1LoopCondition, Le1LoopIter(gamma), ak, s)(n);
+                { Loops.WhileCutTerminatesWithFuelUnroll(Le1LoopCondition, Le1LoopIter(gamma), ak, s, ak', s', n); }
+                !Loops.WhileCutTerminatesWithFuel(Le1LoopCondition, Le1LoopIter(gamma), ak', s')(n - 1);
+                s' in restOfLoopDiverges;
+              }
+            } else {
+              assert s !in divergenceEvent by {
+                calc {
+                  s in divergenceEvent;
+                  !Loops.WhileCutTerminatesWithFuel(Le1LoopCondition, Le1LoopIter(gamma), ak, s)(n);
+                  { Loops.WhileCutTerminatesWithFuelUnroll(Le1LoopCondition, Le1LoopIter(gamma), ak, s, ak', s', n); }
+                  !Loops.WhileCutTerminatesWithFuel(Le1LoopCondition, Le1LoopIter(gamma), ak', s')(n - 1);
+                  false;
+                }
+              }
+              assert s !in firstIterationContinuesEvent;
+            }
+        }
+      }
+      assert Rand.prob(divergenceEvent) == Rand.prob(firstIterationContinuesEvent) * Rand.prob(restOfLoopDiverges) by {
+        assume {:axiom} Independence.IsIndepFunction(Le1LoopIter(gamma)(ak)); // TODO
+        Independence.ResultsIndependent(Le1LoopIter(gamma)(ak), continueValues, restOfLoopDiverges);
+      }
+      assert 0.0 <= Rand.prob(restOfLoopDiverges) <= 1.0 by {
+        Rand.ProbIsProbabilityMeasure();
+        Measures.ProbabilityLe1(restOfLoopDiverges, Rand.eventSpace, Rand.prob);
+      }
+      assert 0.0 <= Rand.prob(firstIterationContinuesEvent) <= 1.0 by {
+        Rand.ProbIsProbabilityMeasure(); Measures.ProbabilityLe1(firstIterationContinuesEvent, Rand.eventSpace, Rand.prob);
+      }
+      if n == 1 {
+        assert Rand.prob(firstIterationContinuesEvent) <= 1.0 / k' as real by {
+          assert firstIterationContinuesEvent == Monad.BitstreamsWithValueIn(Le1LoopIter(gamma)(ak), iset{(true, k')}) by {
+            forall s ensures s in firstIterationContinuesEvent <==> s in Monad.BitstreamsWithValueIn(Le1LoopIter(gamma)(ak), iset{(true, k')}) {}
+          }
+          calc {
+            Rand.prob(firstIterationContinuesEvent);
+            { Le1LoopIterCorrectness(gamma, ak, k'); }
+            gamma.numer as real / (k' * gamma.denom) as real;
+            <=
+            1.0 / k' as real;
+          }
+        }
+        calc {
+          Loops.WhileCutDivergenceProbability(Le1LoopCondition, Le1LoopIter(gamma), ak)(n);
+          Rand.prob(divergenceEvent);
+          Rand.prob(firstIterationContinuesEvent) * Rand.prob(restOfLoopDiverges);
+          <= { RealArith.MulMonotonic(Rand.prob(firstIterationContinuesEvent), Rand.prob(restOfLoopDiverges), 1.0); }
+          Rand.prob(firstIterationContinuesEvent);
+          <=
+          1.0 / k' as real;
+          1.0 / (k + n) as real;
+        }
+        assert Loops.WhileCutDivergenceProbability(Le1LoopCondition, Le1LoopIter(gamma), ak)(n) <= Le1LoopDivergenceProbBound(ak.1)(n);
+      } else {
+        calc {
+          Loops.WhileCutDivergenceProbability(Le1LoopCondition, Le1LoopIter(gamma), ak)(n);
+          Rand.prob(divergenceEvent);
+          Rand.prob(firstIterationContinuesEvent) * Rand.prob(restOfLoopDiverges);
+          <= { RealArith.MulMonotonic(Rand.prob(restOfLoopDiverges), Rand.prob(firstIterationContinuesEvent), 1.0); }
+          Rand.prob(restOfLoopDiverges);
+          Loops.WhileCutDivergenceProbability(Le1LoopCondition, Le1LoopIter(gamma), (true, k'))(n - 1);
+          <= { Le1LoopDivergenceProbabilityBound(gamma, (true, k'), n - 1); }
+          1.0 / (k + n) as real;
+        }
+        assert Loops.WhileCutDivergenceProbability(Le1LoopCondition, Le1LoopIter(gamma), ak)(n) <= Le1LoopDivergenceProbBound(ak.1)(n);
+      }
+      }
+      assert Loops.WhileCutDivergenceProbability(Le1LoopCondition, Le1LoopIter(gamma), ak)(n) <= Le1LoopDivergenceProbBound(ak.1)(n);
+    }
+    assert Loops.WhileCutDivergenceProbability(Le1LoopCondition, Le1LoopIter(gamma), ak)(n) <= Le1LoopDivergenceProbBound(ak.1)(n);
+  }
 
 }
